refactor(library): `list.taken/dropn` ~> `list.take/drop`

library/data/buffer.lean
@@ -90,14 +90,14 @@ def foldl : buffer α → β → (α → β → β) → β
 def rev_iterate : Π (b : buffer α), β → (fin b.size → α → β → β) → β
 | ⟨_, a⟩ b f := a.rev_iterate b f
 
-def taken (b : buffer α) (n : nat) : buffer α :=
-if h : n ≤ b.size then ⟨n, b.to_array.taken n h⟩ else b
+def take (b : buffer α) (n : nat) : buffer α :=
+if h : n ≤ b.size then ⟨n, b.to_array.take n h⟩ else b
 
-def taken_right (b : buffer α) (n : nat) : buffer α :=
-if h : n ≤ b.size then ⟨n, b.to_array.taken_right n h⟩ else b
+def take_right (b : buffer α) (n : nat) : buffer α :=
+if h : n ≤ b.size then ⟨n, b.to_array.take_right n h⟩ else b
 
-def dropn (b : buffer α) (n : nat) : buffer α :=
-if h : n ≤ b.size then ⟨_, b.to_array.dropn n h⟩ else b
+def drop (b : buffer α) (n : nat) : buffer α :=
+if h : n ≤ b.size then ⟨_, b.to_array.drop n h⟩ else b
 
 def reverse (b : buffer α) : buffer α :=
 ⟨b.size, b.to_array.reverse⟩
