library/init/data/array/slice.lean
@@ -16,18 +16,18 @@ def slice (a : array α n) (k l : nat) (h₁ : k ≤ l) (h₂ : l ≤ n) : array
          ... = l : nat.sub_add_cancel h₁
          ... ≤ n : h₂⟩ ⟩
 
-def taken (a : array α n) (m : nat) (h : m ≤ n) : array α m :=
+def take (a : array α n) (m : nat) (h : m ≤ n) : array α m :=
 cast (by simp) $ a.slice 0 m (nat.zero_le _) h
 
-def dropn (a : array α n) (m : nat) (h : m ≤ n) : array α (n-m) :=
+def drop (a : array α n) (m : nat) (h : m ≤ n) : array α (n-m) :=
 a.slice m n h (le_refl _)
 
 private lemma sub_sub_cancel (m n : ℕ) (h : m ≤ n) : n - (n - m) = m :=
 calc n - (n - m) = (n - m) + m - (n - m) : by rw nat.sub_add_cancel; assumption
              ... = m : nat.add_sub_cancel_left _ _
 
-def taken_right (a : array α n) (m : nat) (h : m ≤ n) : array α m :=
-cast (by simp [*, sub_sub_cancel]) $ a.dropn (n - m) (nat.sub_le _ _)
+def take_right (a : array α n) (m : nat) (h : m ≤ n) : array α m :=
+cast (by simp [*, sub_sub_cancel]) $ a.drop (n - m) (nat.sub_le _ _)
 
 def reverse (a : array α n) : array α n :=
 ⟨ λ ⟨ i, hi ⟩, a.read ⟨ n - (i + 1),
