tests/lean/run/mk_byte.lean
@@ -8,12 +8,12 @@ def byte_type := bitvec 8
 def mk_byte (a b : bool) (l : bitvec 6) : byte_type := a :: b :: l
 
 -- Get the third component
-def get_data (byte : byte_type) : bitvec 6 := vector.dropn 2 byte
+def get_data (byte : byte_type) : bitvec 6 := vector.drop 2 byte
 
 lemma get_data_mk_byte {a b : bool} {l : bitvec 6} : get_data (mk_byte a b l) = l :=
 begin
   apply vector.eq,
   unfold mk_byte,
   unfold get_data,
-  simp [to_list_dropn, to_list_cons, list.dropn]
+  simp [to_list_drop, to_list_cons, list.drop]
 end
